git-svn-id: orca@558

C-verifier/src/Midend-IVL/Isabelle-UTP-Extended/hoare/HoareLogic/TotalCorrectness/IMP_Prog/utp_hoare_ndes_prog.thy
@@ -3,8 +3,30 @@ theory utp_hoare_ndes_prog
 imports "../../../AlgebraicLaws/IMP_Prog/algebraic_laws_prog"
 
 begin
+
+section {*Helper*}    
+
+text \<open>The below definition helps in asserting independence for a group of lenses, as otherwise the
+number of assumptions required increases greatly. Unfortunately, it is not usable with lenses of
+different types as Isabelle does not allow heterogenous lists; element types must be unifiable.\<close>
+
+definition \<open>lens_indep_all lenses \<longleftrightarrow> (\<forall>l \<in> set lenses. vwb_lens l \<and> eff_lens l) \<and>
+                                      (\<forall>i j. i < length lenses \<and> j < length lenses \<and>
+                                             i \<noteq> j \<longrightarrow> lenses!i \<bowtie> lenses!j)\<close>
+
+lemma lens_indep_all_alt:
+  \<open>lens_indep_all lenses \<longleftrightarrow> (\<forall>l \<in> set lenses. vwb_lens l \<and> eff_lens l) \<and>
+                              distinct lenses \<and>
+                             (\<forall>a \<in> set lenses. \<forall>b \<in> set lenses. a \<noteq> b \<longrightarrow> a \<bowtie> b)\<close>
+  unfolding lens_indep_all_def distinct_conv_nth
+  apply (safe; simp?)
+   apply (metis lens_indep_quasi_irrefl nth_mem vwb_lens_wb)
+  apply (metis in_set_conv_nth)
+  done
+
 section {*Hoare logic for programs*}  
-named_theorems hoare_prog and hoare_sp_vcg_rule
+
+named_theorems hoare_prog and hoare_sp_vcg_rules
 
 subsection {*Hoare triple definition*}
 
@@ -17,11 +39,11 @@ lemma hoare_true_assisgns_prog_t[hoare_prog]:
   "\<lbrace>p\<rbrace> \<langle>\<sigma>\<rangle>\<^sub>p \<lbrace>true\<rbrace>\<^sub>P"
   by (simp add: prog_rep_eq hoare_des)
 
-lemma hoare_true_skip_prog_t [hoare_prog]: 
-  "\<lbrace>p\<rbrace>skip\<lbrace>true\<rbrace>\<^sub>P"
+lemma hoare_true_skip_prog_t[hoare_prog]: 
+  "\<lbrace>p\<rbrace>SKIP\<lbrace>true\<rbrace>\<^sub>P"
   by (simp add: prog_rep_eq hoare_des)
 
-lemma hoare_false_prog_t [hoare_prog]: 
+lemma hoare_false_prog_t[hoare_prog]: 
   "\<lbrace>false\<rbrace>C\<lbrace>q\<rbrace>\<^sub>P"
   by (simp add: prog_rep_eq hoare_des)
 
@@ -67,7 +89,7 @@ lemma assigns_prog_hoare_prog_backward_t' [hoare_prog]:
   "\<lbrace>\<sigma> \<dagger> p\<rbrace>\<langle>\<sigma>\<rangle>\<^sub>p\<lbrace>p\<rbrace>\<^sub>P"
   by (simp add: prog_rep_eq hoare_des)
 
-lemma assigns_prog_floyd_t [hoare_prog, hoare_sp_vcg_rule]:
+lemma assigns_prog_floyd_t [hoare_prog]:
   assumes "vwb_lens x"
   shows \<open>\<lbrace>p\<rbrace>x :== e\<lbrace>\<^bold>\<exists>v \<bullet> p\<lbrakk>\<guillemotleft>v\<guillemotright>/x\<rbrakk> \<and> &x =\<^sub>u e\<lbrakk>\<guillemotleft>v\<guillemotright>/x\<rbrakk>\<rbrace>\<^sub>P\<close>
   using assms  
@@ -89,6 +111,13 @@ lemma cond_prog_hoare_prog_t [hoare_prog]:
   using assms
   by (simp add: prog_rep_eq hoare_des) 
 
+    
+lemma cond_prog_hoare_prog_t'[hoare_des]:
+  assumes \<open>\<lbrace>b \<and> p\<rbrace>C\<^sub>1\<lbrace>q\<rbrace>\<^sub>P\<close> and \<open>\<lbrace>\<not>b \<and> p\<rbrace>C\<^sub>2\<lbrace>s\<rbrace>\<^sub>P\<close>
+  shows \<open>\<lbrace>p\<rbrace>IF b THEN C\<^sub>1 ELSE C\<^sub>2 FI\<lbrace>q \<or> s\<rbrace>\<^sub>P\<close>
+  using assms
+  by (simp add: prog_rep_eq hoare_des) 
+    
 subsection {*Hoare for recursion*}
 
 lemma mono_Monotone_prog: (*This can be used to generate lemmas automatically*)
@@ -100,7 +129,7 @@ lemma N_prog_funcset: (*This can be used to generate lemmas automatically*)
   "Rep_prog \<circ> F \<circ> Abs_prog \<circ> \<H>\<^bsub>NDES\<^esub> \<in> \<lbrakk>\<^bold>N\<rbrakk>\<^sub>H \<rightarrow> \<lbrakk>\<^bold>N\<rbrakk>\<^sub>H"  
   using Rep_prog by auto
    
-lemma mu_p_rec_hoare_p_t [hoare_prog]:
+lemma mu_prog_rec_hoare_prog_t [hoare_prog]:
   assumes WF: "wf R"
   assumes M:"mono F"  
   assumes induct_step:
@@ -114,14 +143,14 @@ lemma mu_p_rec_hoare_p_t [hoare_prog]:
   apply (simp add: Healthy_if is_Ncarrier_is_ndesigns)
   done
     
-lemma mu_p_rec_hoare_p_t' [hoare_prog]:
+lemma mu_prog_rec_hoare_prog_t' [hoare_prog]:
   assumes WF: "wf R"
   assumes M:"mono F"  
   assumes induct_step:
     "\<And> st P. \<lbrace>Pre \<and>(E,\<guillemotleft>st\<guillemotright>)\<^sub>u\<in>\<^sub>u\<guillemotleft>R\<guillemotright>\<rbrace> P \<lbrace>Post\<rbrace>\<^sub>P \<Longrightarrow> \<lbrace>Pre \<and> E =\<^sub>u \<guillemotleft>st\<guillemotright>\<rbrace> F P \<lbrace>Post\<rbrace>\<^sub>P" 
   assumes I0: "`Pre' \<Rightarrow> Pre`"  
   shows "\<lbrace>Pre'\<rbrace>\<mu>\<^sub>p F \<lbrace>Post\<rbrace>\<^sub>P"
-  by (simp add: hoare_pre_str_p_t[OF I0 mu_p_rec_hoare_p_t[OF WF M induct_step]])
+  by (simp add: hoare_pre_str_prog_t[OF I0 mu_prog_rec_hoare_prog_t[OF WF M induct_step]])
 
 subsection {*Hoare for frames*}
   
@@ -160,6 +189,7 @@ lemma frame_hoare_p_t_stronger[hoare_prog]:
   shows "\<lbrace>p \<and> r\<rbrace> a:\<lbrakk>P\<rbrakk> \<lbrace>q \<and> r\<rbrace>\<^sub>P"
   using assms 
   by (simp add: prog_rep_eq hoare_des)
+    
 lemma blah1: 
   assumes "vwb_lens g'" "vwb_lens l"
    assumes  "l \<bowtie> g'" 
@@ -182,7 +212,7 @@ lemma
   apply (simp add: prog_rep_eq )
    apply rel_auto 
   apply (metis (no_types, lifting) vwb_lens_wb wb_lens.get_put)
-  apply (rule_tac x="get\<^bsub> g'\<^esub> more" in exI) using 8 4 sledgehammer
+  apply (rule_tac x="get\<^bsub> g'\<^esub> more" in exI) using 8 4 
 proof -
   fix ok\<^sub>v :: bool and more :: 'b and ok\<^sub>v' :: bool and x :: 'b
   assume a1: "\<lbrakk>r\<rbrakk>\<^sub>e more"
@@ -221,7 +251,7 @@ qed
     
 subsection {*Hoare for while iteration*}   
 
-lemma while_invr_hoare_p_t [hoare_prog]:
+lemma while_invr_hoare_prog_t [hoare_prog]:
   assumes WF: "wf R"
   assumes I0: "`Pre \<Rightarrow> I`" 
   assumes induct_step:"\<And>e. \<lbrace>b \<and> I \<and> E =\<^sub>u \<guillemotleft>e\<guillemotright>\<rbrace> body \<lbrace>I \<and>(E,\<guillemotleft>e\<guillemotright>)\<^sub>u\<in>\<^sub>u\<guillemotleft>R\<guillemotright>\<rbrace>\<^sub>P"  
@@ -230,7 +260,7 @@ lemma while_invr_hoare_p_t [hoare_prog]:
   unfolding pwhile_inv_prog_def
   by (simp add: prog_rep_eq while_hoare_ndesign_t[unfolded While_inv_ndes_def, OF WF I0  Rep_prog_H1_H3_closed[THEN H1_H3_impl_H2, THEN H1_H2_impl_H1] induct_step[unfolded prog_rep_eq] PHI])
 
-lemma while_invr_vrt_hoare_p_t [hoare_des]:
+lemma while_invr_vrt_hoare_prog_t [hoare_des]:
   assumes WF: "wf R"
   assumes I0: "`Pre \<Rightarrow> I`"
   assumes induct_step:"\<And> st. \<lbrace>b \<and> I \<and> E =\<^sub>u \<guillemotleft>st\<guillemotright>\<rbrace> body \<lbrace>I \<and>(E,\<guillemotleft>st\<guillemotright>)\<^sub>u\<in>\<^sub>u\<guillemotleft>R\<guillemotright>\<rbrace>\<^sub>P"  
@@ -238,13 +268,13 @@ lemma while_invr_vrt_hoare_p_t [hoare_des]:
   shows "\<lbrace>Pre\<rbrace>INVR I VRT \<guillemotleft>R\<guillemotright>  WHILE b DO body OD\<lbrace>Post\<rbrace>\<^sub>P"
   by (simp add: prog_rep_eq while_hoare_ndesign_t[unfolded While_inv_ndes_def, OF WF I0  Rep_prog_H1_H3_closed[THEN H1_H3_impl_H2, THEN H1_H2_impl_H1] induct_step[unfolded prog_rep_eq] PHI])
 
-lemma while_invr_vrt_hoare_p_t' [hoare_des]:
+lemma while_invr_vrt_hoare_prog_t' [hoare_des]:
   assumes WF: "wf R"
   assumes I0: "`Pre \<Rightarrow> I`"     
   assumes induct_step:"\<And>st. \<lbrace>b \<and> I \<and> E =\<^sub>u \<guillemotleft>st\<guillemotright>\<rbrace> body \<lbrace> P st \<rbrace>\<^sub>P"  
   assumes I0': "\<And>st. `P st \<Rightarrow>I \<and> (E,\<guillemotleft>st\<guillemotright>)\<^sub>u\<in>\<^sub>u\<guillemotleft>R\<guillemotright>`"    
   shows "\<lbrace>Pre\<rbrace>INVR I VRT \<guillemotleft>R\<guillemotright>  WHILE b DO body OD\<lbrace>\<not>b \<and> I\<rbrace>\<^sub>P"
-proof (rule while_invr_vrt_hoare_p_t[OF WF I0, of _ E], goal_cases)
+proof (rule while_invr_vrt_hoare_prog_t[OF WF I0, of _ E], goal_cases)
   case (1 st)
   then show ?case using induct_step I0' unfolding prog_rep_eq by pred_blast
 next
@@ -257,41 +287,186 @@ lemma while_invr_hoare_r':
   shows \<open>\<lbrace>pre\<rbrace>while b invr p do C od\<lbrace>\<not>b \<and> p\<rbrace>\<^sub>u\<close>
   by (metis while_inv_def assms hoare_post_weak hoare_pre_str while_hoare_r)
     
-lemmas while_invr_vrt_hoare_p_t_instantiated[hoare_sp_vcg_rule] = 
-       while_invr_vrt_hoare_p_t'[where E = "&\<Sigma>"]
+lemmas while_invr_vrt_hoare_prog_t_instantiated = 
+       while_invr_vrt_hoare_prog_t'[where E = "&\<Sigma>"]
        
 term "(measure o Rep_uexpr) ((&y + 1) - &x)"  
   
 section {*VCG*} 
+lemmas [hoare_sp_vcg_rules] =  
+  assigns_prog_floyd_t seq_hoare_prog_t cond_prog_hoare_prog_t'  
+  while_invr_vrt_hoare_prog_t_instantiated skip_prog_hoare_prog_t
   
-method hoare_sp_vcg_pre = (simp only: seqr_assoc[symmetric])?, rule hoare_post_weak  
+method_setup insert_assms = \<open>Scan.succeed (fn _ => CONTEXT_METHOD (fn facts => fn (ctxt,st) => let
+   val tac = HEADGOAL (Method.insert_tac ctxt facts)
+   val ctxt = Method.set_facts [] ctxt
+ in Method.CONTEXT ctxt (tac st)
+ end))\<close>                      
+        
+(*method insert_assms =  tactic \<open>@{context} |>  Assumption.all_prems_of |> (@{context} |>  Method.insert_tac) |> FIRSTGOAL\<close>*)
+                      
+method hoare_sp_vcg_pre = (simp only: seqr_assoc[symmetric])?, rule hoare_post_weak_prog_t  
 
+method hoare_sp_vcg_rule = rule hoare_sp_vcg_rules
+
+named_theorems lens_laws_vcg_simps
+lemmas [lens_laws_vcg_simps] =
+  lens_indep.lens_put_irr1
+  lens_indep.lens_put_irr2
+  
+method vcg_default_solver = assumption|pred_simp?;(simp add: lens_laws_vcg_simps)?;fail
+  
+method vcg_step_solver methods solver = 
+       (hoare_sp_vcg_rule | solver)
+  
+method hoare_sp_vcg_step_solver = vcg_step_solver \<open>vcg_default_solver\<close>
+
+  
+text {* The defer processing in the sequel was inspired by tutorial5.thy in Peter Lammich course
+        \url{https://bitbucket.org/plammich/certprog_public/downloads/}*}
+  
+definition DEFERRED :: "bool \<Rightarrow> bool" where "DEFERRED P = P"
+lemma DEFERREDD: "DEFERRED P \<Longrightarrow> P" by (auto simp: DEFERRED_def)
+
+method vcg_can_defer =
+  (match conclusion 
+      in "DEFERRED _" \<Rightarrow> fail  -- \<open>Refuse to defer already deferred goals\<close>
+       \<bar>
+         "\<lbrace>_\<rbrace>_\<lbrace>_\<rbrace>\<^sub>P" \<Rightarrow> fail  -- \<open>Refuse to defer Hoare triples (They are no VCs!)\<close>
+       \<bar> 
+         "_" \<Rightarrow> succeed)
+  
+method vcg_defer = (vcg_can_defer, rule DEFERREDD, tactic \<open>FIRSTGOAL defer_tac\<close>)
+
+method  hoare_sp_vcg_step = (hoare_sp_vcg_rule | vcg_defer)
+  
+method  hoare_sp_vcg_steps = hoare_sp_vcg_pre, hoare_sp_vcg_step+ , (unfold DEFERRED_def)
+
+method  hoare_sp_vcg_steps_pp = hoare_sp_vcg_steps; pred_simp?
+  
+method hoare_sp_vcg_all = (hoare_sp_vcg_pre, (hoare_sp_vcg_step_solver| vcg_defer)+, (unfold DEFERRED_def)?)(*This tactic loops because of vcg_defer*)
+ 
 lemma increment_method: 
   assumes "vwb_lens x" "x \<bowtie> y" "vwb_lens y"
   shows  
     "\<lbrace>&y >\<^sub>u 0\<rbrace>
-    x :== 0 ; 
-    INVR &y >\<^sub>u 0 \<and> &y \<ge>\<^sub>u &x 
-    VRT \<guillemotleft>(measure o Rep_uexpr) ((&y + 1) - &x)\<guillemotright> 
-    WHILE &x <\<^sub>u &y DO x:== (&x + 1) OD
-  \<lbrace>&y =\<^sub>u &x\<rbrace>\<^sub>P"
-  apply (rule hoare_post_weak_p_t)
-   apply (rule seq_hoare_p_t)
-    apply (rule assigns_p_floyd_p_t)
-  using assms(1) apply assumption
-   apply (rule while_invr_vrt_hoare_p_t'[where E = "&\<Sigma>"])
-      apply pred_simp
-  using assms(1,2)
-     apply pred_simp 
-     apply (simp add: lens_indep.lens_put_irr2)
-    apply (rule assigns_p_floyd_p_t)
-  using assms(1) 
-    apply assumption
-  using assms unfolding lens_indep_def
-   apply pred_simp 
-   apply linarith 
-  apply pred_simp
+      x :== 0 ; 
+      INVR &y >\<^sub>u 0 \<and> &y \<ge>\<^sub>u &x 
+      VRT \<guillemotleft>(measure o Rep_uexpr) ((&y + 1) - &x)\<guillemotright> 
+      WHILE &x <\<^sub>u &y DO x:== (&x + 1) OD
+    \<lbrace>&y =\<^sub>u &x\<rbrace>\<^sub>P"
+  apply (insert assms) (*Make this automatic*)
+  apply (hoare_sp_vcg_all)    
   done
+    
+subsection {* I want to see the problem of nested existential*}
+  
+lemma  
+  assumes "vwb_lens x" "x \<bowtie> y" "vwb_lens y"
+  shows  
+    "\<lbrace>&y >\<^sub>u 0\<rbrace>
+      x :== 0 ; 
+      INVR &y >\<^sub>u 0 \<and> &y \<ge>\<^sub>u &x 
+      VRT \<guillemotleft>(measure o Rep_uexpr) ((&y + 1) - &x)\<guillemotright> 
+      WHILE &x <\<^sub>u &y DO x:== (&x + 1) OD
+    \<lbrace>&y =\<^sub>u &x\<rbrace>\<^sub>P"
+  apply (insert assms) (*Make this automatic*)
+    apply hoare_sp_vcg_steps
+
+  oops
+  
+lemma ushExE:
+  assumes " \<lbrakk>\<^bold>\<exists> v \<bullet> P\<rbrakk>\<^sub>e a"
+  assumes "\<And> v .  \<lbrakk>P\<rbrakk>\<^sub>e a \<Longrightarrow> Q " 
+  shows Q
+  using assms 
+  by pred_auto
+
+lemma ushExE':
+  assumes "\<lbrakk>\<^bold>\<exists> v \<bullet> Abs_uexpr (\<lambda>st. \<lbrakk>&y\<rbrakk>\<^sub>e st = y\<^sub>0 \<and> 0 < y\<^sub>0)\<lbrakk>\<guillemotleft>v\<guillemotright>/x\<rbrakk> \<and> &x =\<^sub>u 0\<lbrakk>\<guillemotleft>v\<guillemotright>/x\<rbrakk> \<rbrakk>\<^sub>e a"
+  assumes "\<And>v.  \<lbrakk>Abs_uexpr (\<lambda>st. \<lbrakk>&y\<rbrakk>\<^sub>e st = y\<^sub>0 \<and> 0 < y\<^sub>0)\<lbrakk>\<guillemotleft>v\<guillemotright>/x\<rbrakk> \<and> &x =\<^sub>u 0\<lbrakk>\<guillemotleft>v\<guillemotright>/x\<rbrakk>\<rbrakk>\<^sub>e a \<Longrightarrow> Q " 
+  shows Q
+  using assms 
+  by pred_auto
+    
+lemma even_count:
+  assumes "lens_indep_all [i, start, j, endd]"
+  assumes "vwb_lens x" "vwb_lens y" "vwb_lens i" "vwb_lens j"  
+  shows  
+    "\<lbrace>&start =\<^sub>u \<guillemotleft>0::int\<guillemotright> \<and> &endd =\<^sub>u 1\<rbrace>
+      (i :== &start;
+     j :== 0) (* THIS PRIORITY SUCKS! *) ; 
+     INVR &start =\<^sub>u 0 \<and> &endd =\<^sub>u 1 \<and> &j =\<^sub>u ((&i + 1) - &start) div 2 \<and> &i \<le>\<^sub>u &endd \<and> &i \<ge>\<^sub>u &start
+     VRT \<guillemotleft>measure (nat o (Rep_uexpr ((&endd + 1) - &i)))\<guillemotright>
+     WHILE &i <\<^sub>u &endd
+     DO
+       IF &i mod 2 =\<^sub>u 0 
+       THEN j :== (&j + 1)
+       ELSE SKIP 
+       FI;
+      i :== (&i + 1)
+     OD
+    \<lbrace>&j =\<^sub>u 1\<rbrace>\<^sub>P"
+  apply (insert assms) (*Make this automatic*)
+  apply (hoare_sp_vcg_steps; pred_simp?) 
+   apply (unfold lens_indep_all_alt) 
+   apply (simp_all add: lens_laws_vcg_simps)
+  apply (elim disjE conjE) 
+    apply (simp)
+   apply auto[]
+    apply (simp) 
+  apply (simp add: mod_pos_pos_trivial)
+  done
+    
+subsection {* I want to solve the problem of nested existential*}
+   
+term "Abs_uexpr (\<lambda> st. (Rep_uexpr (&y) st)  = y\<^sub>0  \<and> y\<^sub>0 > 0)" 
+term "Abs_uexpr (\<lambda> st. (Rep_uexpr (&y) st) =  y\<^sub>0 \<and> (Rep_uexpr (&x) st) \<le> y\<^sub>0 \<and> y\<^sub>0 > 0)"    
+term "Abs_uexpr (\<lambda> st. (Rep_uexpr (&y) st)  = y\<^sub>0 \<and> (Rep_uexpr (&x) st) = y\<^sub>0) "  
+term "(\<lambda> x \<bullet> &y >\<^sub>u x)  "
+term "((\<lambda> f x. f x) o Rep_uexpr) (&y >\<^sub>u 0)"  
+term "\<guillemotleft>\<lambda> st. x = (Rep_uexpr (&y >\<^sub>u 0) st)\<guillemotright>"
+term "\<guillemotleft>\<lambda> st. y\<^sub>0 = Rep_uexpr (&y) st\<guillemotright> "
+term "(&y >\<^sub>u 0)"  
+
+
+lemma udeduct_tautI': "\<forall> b. \<lbrakk>p\<rbrakk>\<^sub>eb  \<Longrightarrow> `p`"
+  using taut.rep_eq by blast    
+lemma blahblah: 
+  assumes "vwb_lens x" "x \<bowtie> y" "vwb_lens y"
+  shows  
+    "\<lbrace>Abs_uexpr (\<lambda> st. (Rep_uexpr (&y) st) = y\<^sub>0  \<and> y\<^sub>0 > 0)\<rbrace>
+      x :== 0 ; 
+      INVR Abs_uexpr (\<lambda> st. (Rep_uexpr (&y) st) =  y\<^sub>0 \<and> (Rep_uexpr (&x) st) \<le> y\<^sub>0 \<and> y\<^sub>0 > 0)
+      VRT \<guillemotleft>(measure o Rep_uexpr) ((&y + 1) - &x)\<guillemotright> 
+      WHILE &x <\<^sub>u &y DO x:== (&x + 1) OD
+    \<lbrace>Abs_uexpr (\<lambda> st. (Rep_uexpr (&y) st) = y\<^sub>0 \<and> (Rep_uexpr (&x) st) = y\<^sub>0)\<rbrace>\<^sub>P"
+  apply (insert assms) (*Make this automatic*)
+  apply (hoare_sp_vcg_steps; pred_simp?) 
+   apply (unfold lens_indep_all_alt) 
+   apply (simp_all add: lens_laws_vcg_simps)
+  apply (elim disjE conjE) 
+    apply (simp)
+       apply simp
+      apply simp
+     apply (simp add: usubst)
+     apply (rule  udeduct_tautI)
+    apply (rule uintro)
+     apply (erule ushExE)
+     apply (erule ushExE')
+    apply (subst (asm) Abs_uexpr_inverse)
+     apply (subst Abs_uexpr_inverse)
+    
+  find_theorems name:"Abs_uexp"
+    find_theorems name:"Rep_uexp"
+    thm utp_expr.rep_eq
+    apply simp
+     apply pred_simp
+    apply (subst (asm) HOL.eq_commute[symmetric])
+    apply (simp)
+    apply (vcg_default_solver)+
+  apply (hoare_sp_vcg_all) 
+ done    
 (*
 TODO List for next iteration:
 
